\documentclass[12pt]{article}
\usepackage{amsthm,amssymb,amsfonts,amsmath,amstext,systeme}
\usepackage{graphicx,float}
\usepackage{tabularx}

\marginparwidth 0pt
\oddsidemargin -1.2 truecm
\evensidemargin  0pt 
\marginparsep 0pt
\topmargin -2.2truecm
\linespread{1}
\textheight 25.8 truecm
\textwidth 18.5 truecm
\newenvironment{remark}{\noindent{\bf Remark }}{\vspace{0mm}}
\newenvironment{remarks}{\noindent{\bf Remarks }}{\vspace{0mm}}
\newenvironment{question}{\noindent{\bf Question }}{\vspace{0mm}}
\newenvironment{questions}{\noindent{\bf Questions }}{\vspace{0mm}}
\newenvironment{note}{\noindent{\bf Note }}{\vspace{0mm}}
\newenvironment{summary}{\noindent{\bf Summary }}{\vspace{0mm}}
\newenvironment{back}{\noindent{\bf Background}}{\vspace{0mm}}
\newenvironment{conclude}{\noindent{\bf Conclusion}}{\vspace{0mm}}
\newenvironment{concludes}{\noindent{\bf Conclusions}}{\vspace{0mm}}
\newenvironment{dill}{\noindent{\bf Description of Dill's model}}{\vspace{0mm}}
\newenvironment{maths}{\noindent{\bf Mathematics needed}}{\vspace{0mm}}
\newenvironment{inst}{\noindent{\bf Instructions}}{\vspace{0mm}}
\newenvironment{notes}{\noindent{\bf Notes }}{\vspace{0mm}}
\newenvironment{theorem}{\noindent{\bf Theorem }}{\vspace{0mm}}
\newenvironment{example}{\noindent{\bf Example }}{\vspace{0mm}}
\newenvironment{examples}{\noindent{\bf Examples }}{\vspace{0mm}}
\newenvironment{topics}{\noindent{\bf Topics}}{\vspace{0mm}}
\newenvironment{outcomes}{\noindent{\bf Expected Learning Outcomes}}{\vspace{0mm}}
\newenvironment{lemma}{\noindent{\bf Lemma }}{\vspace{0mm}}
\newenvironment{solution}{\noindent{\it Solution}}{\vspace{2mm}}
\newcommand{\ds}{\displaystyle}
\newcommand{\un}{\underline}
\newcommand{\bs}{\boldsymbol}

\begin{document}

\baselineskip 18 pt
\begin{center}
	{\large \bf X sub i}\\
	\vspace{2 mm}

\end{center}
\vspace{0.05cm}

\textbf{Example.} Solve the following equations:
\begin{enumerate}
	\item[(a)] $12(7x + 5) - 4(27x + 8) = 12(x + 2) - 9(2x - 1)$
	\item[(b)] $24(3x + 7) - 15(7x + 2) = 40(x + 3) - 20(8x - 1)$
	\item[(c)] $24(x + 5) + 132(19x + 11) = 88(13x + 2) + 33(2x - 1)$
	\item[(d)] $55(2x + 2) - 33(5x + 7) = 55(13x + 17) - 15(23x - 29)$
	\item[(e)] $45(x + 3) - 63(5x + 9) = 105(2x + 3) - 35(x - 2)$
\end{enumerate}

\vfill

\begin{enumerate}
	\item[(a)] $x = \dfrac{-5}{18}$
	\item[(b)] $x = \dfrac{2}{87}$
	\item[(c)] $x = \dfrac{-1429}{1322}$
	\item[(d)] $x = \dfrac{-1491}{425}$
	\item[(e)] $x = \dfrac{-817}{445}$
\end{enumerate}

\newpage

\textbf{Example.} Solve the following equations:
\begin{enumerate}
	\item[(a)] $\dfrac{7x + 5}{3} - \dfrac{27x + 8}{9} = \dfrac{x + 2}{3} - \dfrac{2x - 1}{4}$
	\item[(b)] $\dfrac{3x + 7}{5} - \dfrac{7x + 2}{8} = \dfrac{x + 3}{3} - \dfrac{8x - 1}{6}$
	\item[(c)] $\dfrac{x + 5}{11} + \dfrac{19x + 11}{2} = \dfrac{13x + 2}{3} + \dfrac{2x - 1}{8}$
	\item[(d)] $\dfrac{2x + 2}{3} - \dfrac{5x + 7}{5} = \dfrac{13x + 17}{3} - \dfrac{23x - 29}{11}$
	\item[(e)] $\dfrac{x + 3}{7} - \dfrac{5x + 9}{5} = \dfrac{2x + 3}{3} - \dfrac{x - 2}{9}$
\end{enumerate}

\vfill

\begin{enumerate}
	\item[(a)] $x = \dfrac{-5}{18}$
	\item[(b)] $x = \dfrac{2}{87}$
	\item[(c)] $x = \dfrac{-1429}{1322}$
	\item[(d)] $x = \dfrac{-1491}{425}$
	\item[(e)] $x = \dfrac{-817}{445}$
\end{enumerate}

\newpage

\textbf{Example.} Solve the following equations:
\begin{enumerate}
	\item[(a)] $\dfrac{7x + 5}{3} - \dfrac{27x + 8}{9} = \dfrac{x + 2}{3} - \dfrac{2x - 1}{4}$
	\item[(b)] $\dfrac{3x + 7}{5} - \dfrac{7x + 2}{8} = \dfrac{x + 3}{3} - \dfrac{8x - 1}{6}$
	\item[(c)] $\dfrac{x + 5}{11} + \dfrac{19x + 11}{2} = \dfrac{13x + 2}{3} + \dfrac{2x - 1}{8}$
	\item[(d)] $\dfrac{2x + 2}{3} - \dfrac{5x + 7}{5} = \dfrac{13x + 17}{3} - \dfrac{23x - 29}{11}$
	\item[(e)] $\dfrac{x + 3}{7} - \dfrac{5x + 9}{5} = \dfrac{2x + 3}{3} - \dfrac{x - 2}{9}$
\end{enumerate}

\vfill

\begin{enumerate}
	\item[(a)] $x = \dfrac{-5}{18}$
	\item[(b)] $x = \dfrac{2}{87}$
	\item[(c)] $x = \dfrac{-1429}{1322}$
	\item[(d)] $x = \dfrac{-1491}{425}$
	\item[(e)] $x = \dfrac{-817}{445}$
\end{enumerate}

\end{document}