\documentclass[12pt]{article}
\usepackage{amsthm,amssymb,amsfonts,amsmath,amstext,systeme}

\marginparwidth 0pt
\oddsidemargin -1.2 truecm
\evensidemargin  0pt 
\marginparsep 0pt
\topmargin -2.2truecm
\linespread{1}
\textheight 25.8 truecm
\textwidth 18.5 truecm
\newenvironment{remark}{\noindent{\bf Remark }}{\vspace{0mm}}
\newenvironment{remarks}{\noindent{\bf Remarks }}{\vspace{0mm}}
\newenvironment{question}{\noindent{\bf Question }}{\vspace{0mm}}
\newenvironment{questions}{\noindent{\bf Questions }}{\vspace{0mm}}
\newenvironment{note}{\noindent{\bf Note }}{\vspace{0mm}}
\newenvironment{summary}{\noindent{\bf Summary }}{\vspace{0mm}}
\newenvironment{back}{\noindent{\bf Background}}{\vspace{0mm}}
\newenvironment{conclude}{\noindent{\bf Conclusion}}{\vspace{0mm}}
\newenvironment{concludes}{\noindent{\bf Conclusions}}{\vspace{0mm}}
\newenvironment{dill}{\noindent{\bf Description of Dill's model}}{\vspace{0mm}}
\newenvironment{maths}{\noindent{\bf Mathematics needed}}{\vspace{0mm}}
\newenvironment{inst}{\noindent{\bf Instructions}}{\vspace{0mm}}
\newenvironment{notes}{\noindent{\bf Notes }}{\vspace{0mm}}
\newenvironment{theorem}{\noindent{\bf Theorem }}{\vspace{0mm}}
\newenvironment{example}{\noindent{\bf Example }}{\vspace{0mm}}
\newenvironment{examples}{\noindent{\bf Examples }}{\vspace{0mm}}
\newenvironment{topics}{\noindent{\bf Topics}}{\vspace{0mm}}
\newenvironment{outcomes}{\noindent{\bf Expected Learning Outcomes}}{\vspace{0mm}}
\newenvironment{lemma}{\noindent{\bf Lemma }}{\vspace{0mm}}
\newenvironment{solution}{\noindent{\it Solution}}{\vspace{2mm}}
\newcommand{\ds}{\displaystyle}
\newcommand{\un}{\underline}
\newcommand{\bs}{\boldsymbol}

\begin{document}

\baselineskip 18 pt
\begin{center}
	{\large \bf Differentiation Exercise}\\
	\vspace{2 mm}
\end{center}
\vspace{0.05cm}


\begin{enumerate}
\item
Use the definition of derivative to compute $f'(x)$ for each of the following.
\begin{enumerate}
\item[(a)]
$f(x) = \sqrt{4x-1}$
\item[(b)]
$f(x) = \sqrt{2 + x^2}$
\item[(c)]
$\ds f(x) = \frac{1}{2x + 1}$
\item[(d)]
$f(x) = \cos x$
\item[(e)]
$f(x) = \tan x$
\item[(f)]
$f(x) = \ln x$
\end{enumerate}

\item
Find $\ds \frac{dy}{dx}$ for each of the following.
\begin{enumerate}
\item[(a)] $\displaystyle{y = -8x^{5}+\sqrt{3}x^{3}+2\pi x^{2}-12}$
\item[(b)] $\displaystyle{y = \left(x^{100}+2x^{50}-3\right)\left(7x^{8}+20x+5\right)}$
\item[(c)] $\displaystyle{y = \frac{x^{5}-x+2}{x^{3}+7}}$
\item[(d)] $\displaystyle{y = \left(x^{3}-2x^{2}+7x-3\right)^{4}}$
\item[(e)] $\displaystyle{y = \frac{1}{\left(3x^{2}+5\right)^{4}}}$
\item[(f)] $\displaystyle y = \sqrt{2x+7}$
\item[(g)] $\displaystyle{y = \left(\frac{x+2}{x-3}\right) ^{3}}$
\item[(h)] $\ds y = x^{\frac{1}{2}}\cos\left( 2x^{3}+x-10\right)$
\item[(j)] $\displaystyle y = \ln\left((\ln x)^5\right)$
\item[(k)] $\displaystyle{y = \sin^{3}(5x+4)}$
\item[(l)] $\displaystyle y = \tan^3(\ln x)$
\item[(m)] $\displaystyle y = \frac{x}{\cos^2(2x)}$
\item[(n)] $\ds y = \sin ^{2}(4x) -4\cos\left(x^{2}-1\right) + \sin(x\ln x)$
\item[(o)] $\ds y = e^{3x^{2}+5x-2}$
\item[(p)] $\ds y = \ln\left(\frac{e^{x}+2x+1}{e^{x}-3x-1}\right)$
\item[(q)] $\ds y = \frac{1}{4}xe^{4x} - \frac{1}{16}e^{4x}$
\item[(r)] $\displaystyle y = \log_x(2x + 3)$
\item[(s)] $\ds y = \sin^{-1}\left(\sqrt{1-x^2}\right)$

\end{enumerate}
\newpage
\item
Find $\ds \frac{dy}{dx}$ for each of the following.
\begin{enumerate}
\item[(a)] $x^2 + y^2 - 4x + 6y + 12 = 0$
\item[(b)] $xy + y^2 = 1$
\item[(c)] $x + \sin y = xy$
\item[(d)] $\tan(xy) = y$
\item[(e)] $y = \tan^2(x+y)$
\item[(f)] $xy^3 - 2x^2 = xy + 5$
\item[(g)] $\ds \sin\left(x^2 + y\right) = 3xy^2 + y^2$
\item[(h)] $x\sqrt{x+y} = 8 - xy$
\item[(i)] $x^2(x-y)^2 = x^2 - y^2$
\item[(j)] $\ds y^2 = \frac{x-1}{x+1}$
\item[(k)] $x^4 = x^2y^2 + 2\ln y$
\item[(l)] $\ds x^2 + y^2 = 2x\cos\left(y^3\right)$
\end{enumerate}

\item
Find $\ds \frac{dy}{dx}$ for each of the following.
\begin{enumerate}
\item[(a)] $\ds y = \sqrt[5]{\frac{x-1}{x+1}}$
\item[(b)] $\ds y = \frac{x^2 \sqrt[3]{7x-14}}{\left(1+x^2\right)^4}$
\item[(c)] $\ds y = \frac{x^{\frac{3}{4}} \sqrt{x^2 + 1}}{(3x+2)^5}$
\item[(d)] $\ds y = \frac{x^3}{1-x} \sqrt[3]{\frac{3-x}{(3+x)^2}}$
\item[(e)] $\ds y = \sqrt[3]{\frac{(x+2)(3x-1)^4}{(2-x)^5}}$
\item[(f)] $\ds y = 2^{\sin x}$
\item[(g)] $\ds y = 3^{\tan\frac{1}{x}}$
\item[(h)] $\ds y = x^{\ln x}$
\item[(i)] $\ds y = (\sin x)^x$
\item[(j)] $\ds y = (1+x)^{\frac{1}{x}}$
\item[(n)] $\ds y = \sin\left(x^{\cos x}\right)$
\end{enumerate}

\item
\begin{enumerate}
\item[(a)]
Given $\displaystyle{y=\frac{u^{2}-1}{u^{2}+1}}$ and $u=\sqrt[3]{x^{2}+2}$, find $\displaystyle{\frac{dy}{dx}}$ in terms of $x$.
\item[(b)]
Given $\displaystyle{y=\frac{1}{\sqrt{3u^2 + 4}}}$ and $u=e^{-x}$, find $\displaystyle{\frac{dy}{dx}}$ in terms of $x$.
\item[(c)]
Given $y = 2x^2 + 1$ and $u=2x-1$, find $\displaystyle{\frac{dy}{du}}$ in terms of $u$.
\end{enumerate}

\item
\begin{enumerate}
\item[(a)]
If $F(x)=f\left(g(x)\right)$, where $f(-2)=8$, $f'(-2)=4$, $f'(5)=3$, $g(5)=-2$ and $g'(5)=6$, find $F'(5)$.
\item[(b)]
Find $f'$ in terms of $g$ and/or $g'$ for each of the following.
\begin{enumerate}
\item[(i)]
$\ds f(x)=\left(g(x)\right)^2$
\item[(ii)]
$\ds f(x) = \sin\left(g(x)\right)$
\item[(iii)]
$\ds f(x) = g(\sin x)$
\end{enumerate}
\item[(c)]
Let $f$ and $g$ be two differentiable functions such that $f\left(g(x)\right)=x$ and $f'(x) = 1 + \left(f(x)\right)^2$. Show that $\ds g'(x)=\frac{1}{1+x^2}$.
\end{enumerate}

\item
\begin{enumerate}
\item[(a)]
Find the equation of the tangent line to the graph of $y = x^2 - \cos x - 1$ at $x = \pi$.
\item[(b)]
Find the points on the curve $y=2x^3+3x^2-12x+1$ at which the tangent lines are horizontal.
\item[(c)]
Find the equations of both lines that are tangent to the curve $y=1+x^3$ and are parallel to the line $12x-y=1$.
\item[(d)]
Find the equations of the tangent lines to the curve $\ds y = \frac{x-1}{x+1}$ that are parallel to the line $x-2y=2$.
\end{enumerate}

\item
\begin{enumerate}
\item[(a)]
For what values of $a$ and $b$ is the line $2x+y=b$ tangent to the curve $y = ax^2$ when $x=2$?
\item[(b)]
For what value(s) of $c$ is the curve $\ds y = \frac{c}{x+1}$ tangent to the line through the points $(0, 3)$ and $(5, -2)$?
\end{enumerate}

\item
The equation of a curve $C$ is $y = x^3 - 2x^2 - 4$.
\begin{enumerate}
\item[(a)]
Find the point(s) on $C$ at which the tangent line(s) to $C$
\begin{enumerate}
\item[(i)]
is/are parallel to the line $4x - y = 3$.
\item[(ii)]
cut(s) the $x$-axis at the point $(-1, 0)$. 
\end{enumerate}
\item[(b)]
Write down the equations of the corresponding tangent lines in (a)(i) and (ii).
\end{enumerate} 

\item
Let $f(x) = 2x^3 + 5x^2 - 12$.
\begin{enumerate}
\item[(a)]
Find the equation of the tangent line to the graph of $y = f(x)$ at $x = 1$.
\item[(b)]
Find the value(s) of $m$ for which the line $y=mx$ is tangent to the graph of $y = f(x)$.
\end{enumerate}

\item
\begin{enumerate}
\item[(a)]
A curve is defined by the equation $2x^4 - 2x^2y^2 - y^3 + 1 = 0$ and $(1, 1)$ is a point on the curve. Find the slope of the tangent line to the curve at this point.
\item[(b)]
Let $C$ be the curve defined by the equation $x = 2y^2 - y^3$. Find the equation(s) of the tangent line(s) to $C$ such that the slope of each tangent line is one.
\end{enumerate}

\item
\begin{enumerate}
\item[(a)]
If $f(x)=x^3+x-9$, find $\left(f^{-1}\right)'(1)$.
\item[(b)]
If $g(x)=2x+\cos x$, find $\left(g^{-1}\right)'(1)$.
\item[(c)]
If $\ds h(x)=\frac{4x^3}{x^2 + 1}$, find $\left(h^{-1}\right)'(2)$.
\end{enumerate}

\item
Let $f$ be a differentiable function such that $f(0) = 3$, $f'(0) = 5$, $f(1) = 7$, $f'(1) = 9$, $\ds f\left(\frac{\pi}{2}\right) = 11$ and $\ds f'\left(\frac{\pi}{2}\right) = 15$.
\begin{enumerate}
\item[(a)]
Compute $g'(7)$, where $\ds g(x) = \frac{1}{f^{-1}(x)}$ and $f^{-1}$ is the inverse function of $f$.
\item[(b)]
Find the derivative of $h$ at $x = 0$, where $\ds h(x) = f\left(\cos^{-1}\frac{x}{3}\right)$.
\end{enumerate}

\item
Find $\ds \frac{dy}{dx}$, $\ds \frac{d^2 y}{dx^2}$ and $\ds \frac{d^3 y}{dx^3}$ for each of the following functions.
\begin{enumerate}
\item[(a)]
$y = \ln x$
\item[(b)]
$\ds y = \frac{1}{ax+b}$, where $a$ and $b$ are constants with $a \ne 0$.
\item[(c)]
$y = e^x(x-1)$
\item[(d)]
$y = \sin^2 x$
\end{enumerate}

\item
Find $\ds \frac{d^2 y}{dx^2}$ in terms of $x$ and $y$ for each of the following. Hence evaluate $\ds \frac{d^2 y}{dx^2}$ at the point $(0,1)$.
\begin{enumerate}
\item[(a)]
$x^2 + 4y^2 = 4$
\item[(b)]
$x^3 - 3xy + y^3 = 1$
\end{enumerate}

\item
\begin{enumerate}
\item[(a)]
If $\ds y = \frac{x+a}{x+b}$, where $a$ and $b$ are constants, show that $\ds 2\left(\frac{dy}{dx}\right)^2 + (1-y)\frac{d^2 y}{dx^2} = 0$.
\item[(b)]
If $\displaystyle y = \frac{1}{\sqrt{1 + x^2}}$, show that $\ds \left(1 + x^2\right)\frac{d^2 y}{dx^2} + 3x\frac{dy}{dx} + y = 0$.
\end{enumerate}





\end{enumerate}










\end{document}